Reorganise code into some more files

LambdaGraph/Basic.lean
@@ -37,143 +37,10 @@ structure Computation extends Program where
   /-- The expression to be evaluated. -/
   expr : Expr
 
-/--
-The free-variable relation.
-
-A variable occurs free in an expression if the expression itself contains the
-variable, or if it contains a reference to a function in which the variable
-occurs free.
--/
-inductive Expr.Free (p : Program) (n : Nat) : Expr → Prop where
-  | var : Free p n (.var n)
-  | fn (m : Nat) (_ : m < p.size) : n ≠ m → Free p n p.fn[m] → Free p n (.fn m)
-  | appL (f e : Expr) : Free p n f → Free p n (.app f e)
-  | appR (f e : Expr) : Free p n e → Free p n (.app f e)
-  | condC (c et ef : Expr) : Free p n c → Free p n (.cond c et ef)
-  | condT (c et ef : Expr) : Free p n et → Free p n (.cond c et ef)
-  | condF (c et ef : Expr) : Free p n ef → Free p n (.cond c et ef)
-
-/--
-The nesting relation between functions in a program.
-
-During substitution, all functions nested in the function corresponding to the
-substitution variable must be rewritten.
--/
-inductive Nests (p : Program) (n : Nat) : Nat → Prop where
-  | free (m : Nat) (_ : m < p.size) : n ≠ m → p.fn[m].Free p n → Nests p n m
-  | step (m k : Nat) (_ : k < p.size) :
-    m ≠ k → p.fn[k].Free p m → Nests p n m → Nests p n k
-
-/-- An expression is closed if it has no free variables. -/
-def Expr.Closed (p : Program) (e : Expr) : Prop := ∀ n, ¬e.Free p n
-
-/--
-Free variables of a computation.
-
-A variable occurs free in a computation if it occurs free in the computation's
-expression.
--/
-def Computation.Free (p : Computation) (n : Nat) := p.expr.Free p.toProgram n
-
-/-- A computation is closed if its expression is closed in its program. -/
-def Computation.Closed (p : Computation) : Prop := ∀ n, ¬p.Free n
-
-/--
-A mapping from old labels to new labels assigned for substitution.
-
-There is also a mapping that maps the newly assigned labels back to their
-original labels.
--/
-structure LabelMap (p : Program) where
-  fwd : Vector Nat p.size
-  inv : Array (Fin p.size)
-
-open Classical in -- TODO: Remove this by implementing Decidable.
-/-- Returns a label map to use for substitution of the variable `n`. -/
-noncomputable def Program.labelMap (p : Program) (n : Nat) :
-    LabelMap p :=
-  let (fwd, inv) := aux 0 (Vector.ofFn Fin.val) #[]
-  ⟨fwd, inv⟩
-where
-  aux i map inv :=
-    if h : i < p.size then
-      if Nests p n i then
-        aux (i + 1) (map.set i (p.size + inv.size)) (inv.push ⟨i, h⟩)
-      else
-        aux (i + 1) map inv
-    else
-      (map, inv)
-
-/--
-Substitutes a value for a variable in an expression.
-
-The expression may include references to functions nested inside the function
-corresponding to the substitution variable. For these functions, new versions
-need to be added to the program, with their bodies substituted in the same way.
-This function does not perform this change to the program, but takes a label map
-mapping function labels to the labels assigned to their substituted versions.
--/
-noncomputable def Expr.subst {p : Program} (e : Expr) (map : LabelMap p)
-    (n : Nat) (v : Expr) : Expr :=
-  match e with
-  | var m => if n = m then v else var (map.fwd[m]?.getD m)
-  | fn m => fn (map.fwd[m]?.getD m)
-  | app f e => (f.subst map n v).app (e.subst map n v)
-  | bool b => bool b
-  | cond c et ef => (c.subst map n v).cond (et.subst map n v) (ef.subst map n v)
-
-/--
-Substitutes a value for a variable in a program.
-
-This creates a new version of each function that depends on `n`, as specified by
-the passed label map.
--/
-noncomputable def Program.subst (p : Program) (map : LabelMap p) (n : Nat) (v : Expr) :
-    Program :=
-  let fnExt : Vector Expr map.inv.size :=
-    ⟨map.inv.map (p.fn[·].subst map n v), by simp⟩
-  let tyExt : Vector Ty map.inv.size :=
-    ⟨map.inv.map (p.ty[·]), by simp⟩
-  { size := _, fn := p.fn ++ fnExt, ty := p.ty ++ tyExt }
-
-/--
-Substitutes a value for a variable in a computation.
-
-This computes the map for translating old labels into new ones and applies the
-substitution to the program and the expression.
--/
-noncomputable def Computation.subst (p : Computation) (n : Nat) (v : Expr) : Computation :=
-  let map := p.labelMap n
-  ⟨p.toProgram.subst map n v, p.expr.subst map n v⟩
-
 /-- A fully reduced expression. -/
 inductive Expr.Value : Expr → Prop where
   | fn n : Value (.fn n)
   | bool b : Value (.bool b)
-
-/-- The small-step reduction relation. -/
-inductive Step : Computation → Computation → Prop where
-  | app (p : Program) (n : Nat) (e : Expr) (_ : n < p.size) :
-    e.Value → Step ⟨p, .app (.fn n) e⟩ (Computation.subst ⟨p, p.fn[n]⟩ n e)
-  | appL (p p' : Program) (f f' e : Expr) :
-    Step ⟨p, f⟩ ⟨p', f'⟩ → Step ⟨p, f.app e⟩ ⟨p', f'.app e⟩
-  | appR (p p' : Program) (f e e' : Expr) :
-    f.Value → Step ⟨p, e⟩ ⟨p', e'⟩ → Step ⟨p, f.app e⟩ ⟨p', f.app e'⟩
-  | condT (p : Program) (et ef : Expr) :
-    Step ⟨p, (.cond (.bool true) et ef)⟩ ⟨p, et⟩
-  | condF (p : Program) (et ef : Expr) :
-    Step ⟨p, (.cond (.bool false) et ef)⟩ ⟨p, ef⟩
-  | condC (p p' : Program) (c c' et ef : Expr) :
-    Step ⟨p, c⟩ ⟨p', c'⟩ → Step ⟨p, c.cond et ef⟩ ⟨p', c'.cond et ef⟩
-
-notation:40 p:41 " ⇒ " p':41 => Step p p'
-
-/-- The reflexive-transitive closure of the reduction relation. -/
-inductive Steps : Computation → Computation → Prop where
-  | refl (p : Computation) : Steps p p
-  | step (p p' p'' : Computation) : Step p p' → Steps p' p'' → Steps p p''
-
-notation:40 p:41 " ⇒* " p':41 => Steps p p'
 
 /--
 The typing relation on expressions.
@@ -213,3 +80,31 @@ structure Computation.Types (p : Computation) (t : Ty) : Prop where
   expr_types : p.toProgram ⊢ p.expr : t
 
 notation:60 "⊢ " p:61 " : " t:61 => Computation.Types p t
+
+theorem value_types_cn {p : Program} {v : Expr} {t : Ty} (h : p ⊢ v : t.cn) :
+    v.Value → ∃ n, v = .fn n
+  | .fn n => by simp
+  | .bool b => nomatch h
+
+theorem value_types_bool {p : Program} {v : Expr} (h : p ⊢ v : .bool) :
+    v.Value → ∃ b, v = .bool b
+  | .fn n => nomatch h
+  | .bool b => by simp
+
+inductive Expr.ValidRefs (p : Program) : Expr → Prop where
+  | var (n : Nat) : n < p.size → (Expr.var n).ValidRefs p
+  | fn (n : Nat) : n < p.size → (Expr.fn n).ValidRefs p
+  | app (f e : Expr) : f.ValidRefs p → e.ValidRefs p → (f.app e).ValidRefs p
+  | bool (b : Bool) : (Expr.bool b).ValidRefs p
+  | cond (c et ef : Expr) : c.ValidRefs p → et.ValidRefs p → ef.ValidRefs p →
+    (c.cond et ef).ValidRefs p
+
+theorem Expr.Types.validRefs {p : Program} {e : Expr} {t : Ty} (ht : p ⊢ e : t)
+    : e.ValidRefs p := by
+  induction ht with constructor <;> assumption
+
+def Program.ValidRefs (p : Program) : Prop :=
+  ∀ {i} (_ : i < p.size), p.fn[i].ValidRefs p
+
+theorem Program.Types.validRefs {p : Program} (ht : ⊢ p) : p.ValidRefs :=
+  fun hi => (ht hi).validRefs
