LambdaGraph/Subst.lean
@@ -1,69 +1,73 @@
-import LambdaGraph.Basic
+import LambdaGraph.Nest
 
-@[simp]
-theorem not_closed_var {p : Program} {n : Nat} : ¬(Expr.var n).Closed p :=
-  fun h => h n .var
+/--
+A mapping from old labels to new labels assigned for substitution.
 
-theorem fn_closed_iff {p : Program} {m : Nat} :
-    (Expr.fn m).Closed p ↔ ∀ n ≠ m, (_ : m < p.size) → ¬p.fn[m].Free p n := by
-  constructor
-  · intro hc n hn _
-    intro hne
-    solve_by_elim
-  · intro hf n hn
-    cases hn with
-    | fn _ _ hne hn =>
-      solve_by_elim
+There is also a mapping that maps the newly assigned labels back to their
+original labels.
+-/
+structure LabelMap (p : Program) where
+  fwd : Vector Nat p.size
+  inv : Array (Fin p.size)
 
-@[simp]
-theorem app_closed_iff {p : Program} {f e : Expr} :
-    (f.app e).Closed p ↔ f.Closed p ∧ e.Closed p := by
-  constructor
-  · intro h
-    constructor <;> solve_by_elim [Expr.Free.appL, Expr.Free.appR]
-  · rintro ⟨hf, he⟩ n (- | -) <;> solve_by_elim
+open Classical in -- TODO: Remove this by implementing Decidable.
+/-- Returns a label map to use for substitution of the variable `n`. -/
+noncomputable def Program.labelMap (p : Program) (n : Nat) :
+    LabelMap p :=
+  let (fwd, inv) := aux 0 (Vector.ofFn Fin.val) #[]
+  ⟨fwd, inv⟩
+where
+  aux i map inv :=
+    if h : i < p.size then
+      if Nests p n i then
+        aux (i + 1) (map.set i (p.size + inv.size)) (inv.push ⟨i, h⟩)
+      else
+        aux (i + 1) map inv
+    else
+      (map, inv)
 
-@[simp]
-theorem bool_closed (p : Program) (b : Bool) : (Expr.bool b).Closed p := nofun
+/--
+Substitutes a value for a variable in an expression.
 
-@[simp]
-theorem cond_closed_iff {p : Program} {c et ef : Expr} :
-    (c.cond et ef).Closed p ↔ c.Closed p ∧ et.Closed p ∧ ef.Closed p := by
-  constructor
-  · intro h
-    open Expr.Free in
-    and_intros <;> solve_by_elim [condC, condT, condF]
-  · rintro ⟨hc, het, hef⟩ n (- | - | -) <;> solve_by_elim
+The expression may include references to functions nested inside the function
+corresponding to the substitution variable. For these functions, new versions
+need to be added to the program, with their bodies substituted in the same way.
+This function does not perform this change to the program, but takes a label map
+mapping function labels to the labels assigned to their substituted versions.
+-/
+noncomputable def Expr.subst {p : Program} (e : Expr) (map : LabelMap p)
+    (n : Nat) (v : Expr) : Expr :=
+  match e with
+  | var m => if n = m then v else var (map.fwd[m]?.getD m)
+  | fn m => fn (map.fwd[m]?.getD m)
+  | app f e => (f.subst map n v).app (e.subst map n v)
+  | bool b => bool b
+  | cond c et ef => (c.subst map n v).cond (et.subst map n v) (ef.subst map n v)
 
-theorem value_types_cn {p : Program} {v : Expr} {t : Ty} (h : p ⊢ v : t.cn) :
-    v.Value → ∃ n, v = .fn n
-  | .fn n => by simp
-  | .bool b => nomatch h
+/--
+Substitutes a value for a variable in a program.
 
-theorem value_types_bool {p : Program} {v : Expr} (h : p ⊢ v : .bool) :
-    v.Value → ∃ b, v = .bool b
-  | .fn n => nomatch h
-  | .bool b => by simp
+This creates a new version of each function that depends on `n`, as specified by
+the passed label map.
+-/
+noncomputable def Program.subst (p : Program) (map : LabelMap p) (n : Nat)
+    (v : Expr) : Program :=
+  let fnExt : Vector Expr map.inv.size :=
+    ⟨map.inv.map (p.fn[·].subst map n v), by simp⟩
+  let tyExt : Vector Ty map.inv.size :=
+    ⟨map.inv.map (p.ty[·]), by simp⟩
+  { size := _, fn := p.fn ++ fnExt, ty := p.ty ++ tyExt }
 
-theorem size_le_of_step {p p' : Computation} (h : p ⇒ p') :
-    p.size ≤ p'.size := by
-  induction h with simp [*, Program.subst, Computation.subst]
+/--
+Substitutes a value for a variable in a computation.
 
-theorem lt_size_of_step {p p' : Computation} {n : Nat} (hn : n < p.size)
-    (h : p ⇒ p') : n < p'.size := Nat.lt_of_lt_of_le hn (size_le_of_step h)
-
-theorem fn_eq_of_step {p p' : Computation} {n : Nat} (hn : n < p.size)
-    (h : p ⇒ p') : p.fn[n] = p'.fn[n]'(lt_size_of_step hn h) := by
-  induction h with simp [*, Program.subst, Computation.subst]
-
-theorem ty_eq_of_step {p p' : Computation} {n : Nat} (hn : n < p.size)
-    (h : p ⇒ p') : p.ty[n] = p'.ty[n]'(lt_size_of_step hn h) := by
-  induction h with simp [*, Program.subst, Computation.subst]
-
-theorem types_of_step {p p' : Computation} {e : Expr} {t : Ty}
-    (ht : p.toProgram ⊢ e : t) (hs : p ⇒ p') : p'.toProgram ⊢ e : t := by
-  induction ht with
-    (try rw [ty_eq_of_step ‹_› hs]) <;> constructor <;> assumption
+This computes the map for translating old labels into new ones and applies the
+substitution to the program and the expression.
+-/
+noncomputable def Computation.subst (p : Computation) (n : Nat) (v : Expr) :
+    Computation :=
+  let map := p.labelMap n
+  ⟨p.toProgram.subst map n v, p.expr.subst map n v⟩
 
 theorem program_subst_size_le {p : Program} {v : Expr} {n : Nat}
     {map : LabelMap p} : p.size ≤ (p.subst map n v).size := by
@@ -93,15 +97,6 @@ theorem expr_types_in_subst {p : Program} {e : Expr} (v : Expr) {t : Ty}
   | fn m hm =>
     rw [← subst_ty_eq v map hm]
     constructor
-
-theorem Nests.lt {p : Program} {m n : Nat} : Nests p n m → m < p.size
-  | free _ hm _ _ => hm
-  | step _ _ hm _ _ _ => hm
-
-theorem nests_self {p : Program} {n : Nat} :
-    (h : Nests p n n) → ∃ m ≠ n, (p.fn[n]'h.lt).Free p m
-  | .free _ _ hne _ => nomatch hne
-  | .step k _ _ hne hf _ => ⟨k, hne, hf⟩
 
 structure LabelMap.ValidNew {p : Program} (map : LabelMap p) {i : Nat}
     (h : i < p.size) : Prop where
@@ -274,28 +269,6 @@ theorem subst_types {p : Program} {e v : Expr} {t : Ty} {n : Nat}
       simp [hm']
       exact expr_subst_types (labelMap_valid _ hn) (htp _) htv
   · exact expr_subst_types (labelMap_valid _ hn) ht htv
-
-inductive Expr.ValidRefs (p : Program) : Expr → Prop where
-  | var (n : Nat) : n < p.size → (Expr.var n).ValidRefs p
-  | fn (n : Nat) : n < p.size → (Expr.fn n).ValidRefs p
-  | app (f e : Expr) : f.ValidRefs p → e.ValidRefs p → (f.app e).ValidRefs p
-  | bool (b : Bool) : (Expr.bool b).ValidRefs p
-  | cond (c et ef : Expr) : c.ValidRefs p → et.ValidRefs p → ef.ValidRefs p →
-    (c.cond et ef).ValidRefs p
-
-theorem Expr.Types.validRefs {p : Program} {e : Expr} {t : Ty} (ht : p ⊢ e : t)
-    : e.ValidRefs p := by
-  induction ht with constructor <;> assumption
-
-def Program.ValidRefs (p : Program) : Prop :=
-  ∀ {i} (_ : i < p.size), p.fn[i].ValidRefs p
-
-theorem Program.Types.validRefs {p : Program} (ht : ⊢ p) : p.ValidRefs :=
-  fun hi => (ht hi).validRefs
-
-theorem lt_size_of_free {p : Program} {e : Expr} {n : Nat} (hp : p.ValidRefs)
-    (he : e.ValidRefs p) (hf : e.Free p n) : n < p.size := by
-  induction hf with cases he <;> apply_rules
 
 theorem subst_eq_var {p : Program} {e v : Expr} {m n : Nat}
     {map : LabelMap p} (he : e.ValidRefs p) (hc : v.Closed p)
@@ -514,140 +487,3 @@ theorem eq_map_of_free_in_subst {p : Program} {e v : Expr} {m n : Nat}
     have .cond _ _ _ hc het hef := he
     obtain ⟨i, rfl, hf'⟩ := ih hef rfl
     exact ⟨i, rfl, .condF _ _ _ hf'⟩
-
-theorem closed_of_step {p p' : Computation} {e : Expr} (hp : p.ValidRefs)
-    (he : e.ValidRefs p.toProgram) (hc : e.Closed p.toProgram) (hs : p ⇒ p') :
-    e.Closed p'.toProgram := by
-  intro m hf
-  apply hc m
-  induction hs with
-    dsimp only at * <;> apply_rules
-  | app =>
-    dsimp only [Computation.subst] at *
-    exact free_of_free_in_subst hp he hf
-
-theorem progress {p : Computation} {t : Ty} (ht : ⊢ p : t) (hc : p.Closed) :
-    p.expr.Value ∨ ∃ p', p ⇒ p' := by
-  obtain ⟨p, e⟩ := p
-  obtain ⟨htp, hte⟩ := ht
-  simp only at *
-  induction hte with
-  | var n hn => exfalso; exact hc n .var
-  | fn n hn => left; constructor
-  | app f e t htf hte ihf ihe =>
-    right
-    obtain ⟨hcf, hce⟩ := app_closed_iff.mp hc
-    rcases ihf hcf with hvf | ⟨p', hp⟩
-    · rcases ihe hce with hve | ⟨p', hp⟩
-      · obtain ⟨n, rfl⟩ := value_types_cn htf hvf
-        cases htf
-        solve_by_elim [Exists.intro]
-      · exact ⟨_, Step.appR _ _ _ _ _ hvf hp⟩
-    · exact ⟨_, Step.appL _ _ _ _ _ hp⟩
-  | bool b => left; constructor
-  | cond c et ef t htc htet htef ihc ihet ihef =>
-    right
-    obtain ⟨hcc, hcet, hcef⟩ := cond_closed_iff.mp hc
-    rcases ihc hcc with hvc | ⟨p', hp⟩
-    · rcases value_types_bool htc hvc with ⟨_ | _, rfl⟩ <;> repeat constructor
-    · exact ⟨_, Step.condC _ _ _ _ _ _ hp⟩
-
-theorem preservation_types {p p' : Computation} {t : Ty} (ht : ⊢ p : t)
-  (hs : p ⇒ p') : ⊢ p' : t := by
-  obtain ⟨htp, ht⟩ := ht
-  induction hs generalizing t with
-  | app p n e h hv =>
-    have .app _ _ t htf hte := ht
-    cases htf
-    solve_by_elim [subst_types]
-  | appL p p' f f' e hs ih =>
-    have .app _ _ t htf hte := ht
-    obtain ⟨htp', htf'⟩ := ih htp htf
-    constructor
-    · exact htp'
-    · dsimp only at *
-      constructor
-      · exact htf'
-      · exact types_of_step hte hs
-  | appR p p' f e e' hvf hs ih =>
-    have .app _ _ t htf hte := ht
-    obtain ⟨htp', hte'⟩ := ih htp hte
-    constructor
-    · exact htp'
-    · dsimp only at *
-      constructor
-      · exact types_of_step htf hs
-      · exact hte'
-  | condT p et ef => cases ht; constructor <;> assumption
-  | condF p et ef => cases ht; constructor <;> assumption
-  | condC p p' c c' et ef hs ih =>
-    have .cond _ _ _ _ htc htet htef := ht
-    obtain ⟨htp', htc'⟩ := ih htp htc
-    constructor
-    · exact htp'
-    · dsimp only at *
-      constructor
-      · exact htc'
-      · exact types_of_step htet hs
-      · exact types_of_step htef hs
-
-theorem preservation_closed {p p' : Computation} {t : Ty} (ht : ⊢ p : t)
-    (hc : p.Closed) (hs : p ⇒ p') : p'.Closed := by
-  obtain ⟨htp, ht⟩ := ht
-  induction hs generalizing t with
-  | app p n e hn hve =>
-    intro m hm
-    obtain ⟨hcf, hce⟩ := app_closed_iff.mp hc
-    have .app _ _ t' htf hte := ht
-    have hmap : (p.labelMap n).Valid n := labelMap_valid _ hn
-    have hp : p.ValidRefs := htp.validRefs
-    have hfn := hp hn
-    have he := hte.validRefs
-    have hne : n ≠ m := by
-      intro rfl
-      simp [Computation.subst, Computation.Free] at hm
-      exact not_free_in_subst hmap hp hfn he hce hve hm
-    obtain ⟨⟨i, hi⟩, rfl, hf⟩ :=
-      eq_map_of_free_in_subst hmap hp hfn he hce hve hm
-    simp only [Fin.getElem_fin] at hne
-    simp only at hf
-    have hd : ¬Nests p n n := by
-      intro hd
-      obtain ⟨m, hm, hf⟩ := nests_self hd
-      exact hcf m (.fn _ _ hm hf)
-    have hne : i ≠ n := by
-      intro rfl
-      simp [hmap.not_nests hi hd] at hne
-    exact hcf i (.fn _ hn hne hf)
-  | appL p p' f f' e hs ih =>
-    obtain ⟨hcf, hce⟩ := app_closed_iff.mp hc
-    apply app_closed_iff.mpr
-    have .app _ _ t' htf hte := ht
-    dsimp only at *
-    constructor
-    · exact ih hcf htp htf
-    · exact closed_of_step htp.validRefs hte.validRefs hce hs
-  | appR p p' f e e' hvf hs ih =>
-    obtain ⟨hcf, hce⟩ := app_closed_iff.mp hc
-    apply app_closed_iff.mpr
-    have .app _ _ t' htf hte := ht
-    dsimp only at *
-    constructor
-    · exact closed_of_step htp.validRefs htf.validRefs hcf hs
-    · exact ih hce htp hte
-  | condT p et ef =>
-    obtain ⟨-, hcet, -⟩ := cond_closed_iff.mp hc
-    exact hcet
-  | condF p et ef =>
-    obtain ⟨-, -, hcef⟩ := cond_closed_iff.mp hc
-    exact hcef
-  | condC p p' c c' et ef hs ih =>
-    obtain ⟨hcc, hcet, hcef⟩ := cond_closed_iff.mp hc
-    apply cond_closed_iff.mpr
-    have .cond _ _ _ _ htc htet htef := ht
-    and_intros
-    · exact ih hcc htp htc
-    · apply closed_of_step htp.validRefs htet.validRefs hcet
-      exact (.condC _ _ _ _ _ _ hs)
-    · apply closed_of_step htp.validRefs htef.validRefs hcef
-      exact (.condC _ _ _ _ _ _ hs)
