LambdaGraph.lean
@@ -1,4 +1,6 @@
 -- This module serves as the root of the `LambdaGraph` library.
 -- Import modules here that should be built as part of the library.
 import LambdaGraph.Basic
-import LambdaGraph.Lemmas
+import LambdaGraph.Nest
+import LambdaGraph.Subst
+import LambdaGraph.Step
