LambdaGraph/Nest.lean
@@ -1,0 +1,90 @@
+import LambdaGraph.Basic
+
+/--
+The free-variable relation.
+
+A variable occurs free in an expression if the expression itself contains the
+variable, or if it contains a reference to a function in which the variable
+occurs free.
+-/
+inductive Expr.Free (p : Program) (n : Nat) : Expr → Prop where
+  | var : Free p n (.var n)
+  | fn (m : Nat) (_ : m < p.size) : n ≠ m → Free p n p.fn[m] → Free p n (.fn m)
+  | appL (f e : Expr) : Free p n f → Free p n (.app f e)
+  | appR (f e : Expr) : Free p n e → Free p n (.app f e)
+  | condC (c et ef : Expr) : Free p n c → Free p n (.cond c et ef)
+  | condT (c et ef : Expr) : Free p n et → Free p n (.cond c et ef)
+  | condF (c et ef : Expr) : Free p n ef → Free p n (.cond c et ef)
+
+/--
+The nesting relation between functions in a program.
+
+During substitution, all functions nested in the function corresponding to the
+substitution variable must be rewritten.
+-/
+inductive Nests (p : Program) (n : Nat) : Nat → Prop where
+  | free (m : Nat) (_ : m < p.size) : n ≠ m → p.fn[m].Free p n → Nests p n m
+  | step (m k : Nat) (_ : k < p.size) :
+    m ≠ k → p.fn[k].Free p m → Nests p n m → Nests p n k
+
+/-- An expression is closed if it has no free variables. -/
+def Expr.Closed (p : Program) (e : Expr) : Prop := ∀ n, ¬e.Free p n
+
+/--
+Free variables of a computation.
+
+A variable occurs free in a computation if it occurs free in the computation's
+expression.
+-/
+def Computation.Free (p : Computation) (n : Nat) := p.expr.Free p.toProgram n
+
+/-- A computation is closed if its expression is closed in its program. -/
+def Computation.Closed (p : Computation) : Prop := ∀ n, ¬p.Free n
+
+@[simp]
+theorem not_closed_var {p : Program} {n : Nat} : ¬(Expr.var n).Closed p :=
+  fun h => h n .var
+
+theorem fn_closed_iff {p : Program} {m : Nat} :
+    (Expr.fn m).Closed p ↔ ∀ n ≠ m, (_ : m < p.size) → ¬p.fn[m].Free p n := by
+  constructor
+  · intro hc n hn _
+    intro hne
+    solve_by_elim
+  · intro hf n hn
+    cases hn with
+    | fn _ _ hne hn =>
+      solve_by_elim
+
+@[simp]
+theorem app_closed_iff {p : Program} {f e : Expr} :
+    (f.app e).Closed p ↔ f.Closed p ∧ e.Closed p := by
+  constructor
+  · intro h
+    constructor <;> solve_by_elim [Expr.Free.appL, Expr.Free.appR]
+  · rintro ⟨hf, he⟩ n (- | -) <;> solve_by_elim
+
+@[simp]
+theorem bool_closed (p : Program) (b : Bool) : (Expr.bool b).Closed p := nofun
+
+@[simp]
+theorem cond_closed_iff {p : Program} {c et ef : Expr} :
+    (c.cond et ef).Closed p ↔ c.Closed p ∧ et.Closed p ∧ ef.Closed p := by
+  constructor
+  · intro h
+    open Expr.Free in
+    and_intros <;> solve_by_elim [condC, condT, condF]
+  · rintro ⟨hc, het, hef⟩ n (- | - | -) <;> solve_by_elim
+
+theorem lt_size_of_free {p : Program} {e : Expr} {n : Nat} (hp : p.ValidRefs)
+    (he : e.ValidRefs p) (hf : e.Free p n) : n < p.size := by
+  induction hf with cases he <;> apply_rules
+
+theorem Nests.lt {p : Program} {m n : Nat} : Nests p n m → m < p.size
+  | free _ hm _ _ => hm
+  | step _ _ hm _ _ _ => hm
+
+theorem nests_self {p : Program} {n : Nat} :
+    (h : Nests p n n) → ∃ m ≠ n, (p.fn[n]'h.lt).Free p m
+  | .free _ _ hne _ => nomatch hne
+  | .step k _ _ hne hf _ => ⟨k, hne, hf⟩
