LambdaGraph/Step.lean
@@ -1,0 +1,182 @@
+import LambdaGraph.Subst
+
+/-- The small-step reduction relation. -/
+inductive Step : Computation → Computation → Prop where
+  | app (p : Program) (n : Nat) (e : Expr) (_ : n < p.size) :
+    e.Value → Step ⟨p, .app (.fn n) e⟩ (Computation.subst ⟨p, p.fn[n]⟩ n e)
+  | appL (p p' : Program) (f f' e : Expr) :
+    Step ⟨p, f⟩ ⟨p', f'⟩ → Step ⟨p, f.app e⟩ ⟨p', f'.app e⟩
+  | appR (p p' : Program) (f e e' : Expr) :
+    f.Value → Step ⟨p, e⟩ ⟨p', e'⟩ → Step ⟨p, f.app e⟩ ⟨p', f.app e'⟩
+  | condT (p : Program) (et ef : Expr) :
+    Step ⟨p, (.cond (.bool true) et ef)⟩ ⟨p, et⟩
+  | condF (p : Program) (et ef : Expr) :
+    Step ⟨p, (.cond (.bool false) et ef)⟩ ⟨p, ef⟩
+  | condC (p p' : Program) (c c' et ef : Expr) :
+    Step ⟨p, c⟩ ⟨p', c'⟩ → Step ⟨p, c.cond et ef⟩ ⟨p', c'.cond et ef⟩
+
+notation:40 p:41 " ⇒ " p':41 => Step p p'
+
+/-- The reflexive-transitive closure of the reduction relation. -/
+inductive Steps : Computation → Computation → Prop where
+  | refl (p : Computation) : Steps p p
+  | step (p p' p'' : Computation) : Step p p' → Steps p' p'' → Steps p p''
+
+notation:40 p:41 " ⇒* " p':41 => Steps p p'
+
+theorem size_le_of_step {p p' : Computation} (h : p ⇒ p') :
+    p.size ≤ p'.size := by
+  induction h with simp [*, Program.subst, Computation.subst]
+
+theorem lt_size_of_step {p p' : Computation} {n : Nat} (hn : n < p.size)
+    (h : p ⇒ p') : n < p'.size := Nat.lt_of_lt_of_le hn (size_le_of_step h)
+
+theorem fn_eq_of_step {p p' : Computation} {n : Nat} (hn : n < p.size)
+    (h : p ⇒ p') : p.fn[n] = p'.fn[n]'(lt_size_of_step hn h) := by
+  induction h with simp [*, Program.subst, Computation.subst]
+
+theorem ty_eq_of_step {p p' : Computation} {n : Nat} (hn : n < p.size)
+    (h : p ⇒ p') : p.ty[n] = p'.ty[n]'(lt_size_of_step hn h) := by
+  induction h with simp [*, Program.subst, Computation.subst]
+
+theorem types_of_step {p p' : Computation} {e : Expr} {t : Ty}
+    (ht : p.toProgram ⊢ e : t) (hs : p ⇒ p') : p'.toProgram ⊢ e : t := by
+  induction ht with
+    (try rw [ty_eq_of_step ‹_› hs]) <;> constructor <;> assumption
+
+theorem closed_of_step {p p' : Computation} {e : Expr} (hp : p.ValidRefs)
+    (he : e.ValidRefs p.toProgram) (hc : e.Closed p.toProgram) (hs : p ⇒ p') :
+    e.Closed p'.toProgram := by
+  intro m hf
+  apply hc m
+  induction hs with
+    dsimp only at * <;> apply_rules
+  | app =>
+    dsimp only [Computation.subst] at *
+    exact free_of_free_in_subst hp he hf
+
+theorem progress {p : Computation} {t : Ty} (ht : ⊢ p : t) (hc : p.Closed) :
+    p.expr.Value ∨ ∃ p', p ⇒ p' := by
+  obtain ⟨p, e⟩ := p
+  obtain ⟨htp, hte⟩ := ht
+  simp only at *
+  induction hte with
+  | var n hn => exfalso; exact hc n .var
+  | fn n hn => left; constructor
+  | app f e t htf hte ihf ihe =>
+    right
+    obtain ⟨hcf, hce⟩ := app_closed_iff.mp hc
+    rcases ihf hcf with hvf | ⟨p', hp⟩
+    · rcases ihe hce with hve | ⟨p', hp⟩
+      · obtain ⟨n, rfl⟩ := value_types_cn htf hvf
+        cases htf
+        solve_by_elim [Exists.intro]
+      · exact ⟨_, Step.appR _ _ _ _ _ hvf hp⟩
+    · exact ⟨_, Step.appL _ _ _ _ _ hp⟩
+  | bool b => left; constructor
+  | cond c et ef t htc htet htef ihc ihet ihef =>
+    right
+    obtain ⟨hcc, hcet, hcef⟩ := cond_closed_iff.mp hc
+    rcases ihc hcc with hvc | ⟨p', hp⟩
+    · rcases value_types_bool htc hvc with ⟨_ | _, rfl⟩ <;> repeat constructor
+    · exact ⟨_, Step.condC _ _ _ _ _ _ hp⟩
+
+theorem preservation_types {p p' : Computation} {t : Ty} (ht : ⊢ p : t)
+  (hs : p ⇒ p') : ⊢ p' : t := by
+  obtain ⟨htp, ht⟩ := ht
+  induction hs generalizing t with
+  | app p n e h hv =>
+    have .app _ _ t htf hte := ht
+    cases htf
+    solve_by_elim [subst_types]
+  | appL p p' f f' e hs ih =>
+    have .app _ _ t htf hte := ht
+    obtain ⟨htp', htf'⟩ := ih htp htf
+    constructor
+    · exact htp'
+    · dsimp only at *
+      constructor
+      · exact htf'
+      · exact types_of_step hte hs
+  | appR p p' f e e' hvf hs ih =>
+    have .app _ _ t htf hte := ht
+    obtain ⟨htp', hte'⟩ := ih htp hte
+    constructor
+    · exact htp'
+    · dsimp only at *
+      constructor
+      · exact types_of_step htf hs
+      · exact hte'
+  | condT p et ef => cases ht; constructor <;> assumption
+  | condF p et ef => cases ht; constructor <;> assumption
+  | condC p p' c c' et ef hs ih =>
+    have .cond _ _ _ _ htc htet htef := ht
+    obtain ⟨htp', htc'⟩ := ih htp htc
+    constructor
+    · exact htp'
+    · dsimp only at *
+      constructor
+      · exact htc'
+      · exact types_of_step htet hs
+      · exact types_of_step htef hs
+
+theorem preservation_closed {p p' : Computation} {t : Ty} (ht : ⊢ p : t)
+    (hc : p.Closed) (hs : p ⇒ p') : p'.Closed := by
+  obtain ⟨htp, ht⟩ := ht
+  induction hs generalizing t with
+  | app p n e hn hve =>
+    intro m hm
+    obtain ⟨hcf, hce⟩ := app_closed_iff.mp hc
+    have .app _ _ t' htf hte := ht
+    have hmap : (p.labelMap n).Valid n := labelMap_valid _ hn
+    have hp : p.ValidRefs := htp.validRefs
+    have hfn := hp hn
+    have he := hte.validRefs
+    have hne : n ≠ m := by
+      intro rfl
+      simp [Computation.subst, Computation.Free] at hm
+      exact not_free_in_subst hmap hp hfn he hce hve hm
+    obtain ⟨⟨i, hi⟩, rfl, hf⟩ :=
+      eq_map_of_free_in_subst hmap hp hfn he hce hve hm
+    simp only [Fin.getElem_fin] at hne
+    simp only at hf
+    have hd : ¬Nests p n n := by
+      intro hd
+      obtain ⟨m, hm, hf⟩ := nests_self hd
+      exact hcf m (.fn _ _ hm hf)
+    have hne : i ≠ n := by
+      intro rfl
+      simp [hmap.not_nests hi hd] at hne
+    exact hcf i (.fn _ hn hne hf)
+  | appL p p' f f' e hs ih =>
+    obtain ⟨hcf, hce⟩ := app_closed_iff.mp hc
+    apply app_closed_iff.mpr
+    have .app _ _ t' htf hte := ht
+    dsimp only at *
+    constructor
+    · exact ih hcf htp htf
+    · exact closed_of_step htp.validRefs hte.validRefs hce hs
+  | appR p p' f e e' hvf hs ih =>
+    obtain ⟨hcf, hce⟩ := app_closed_iff.mp hc
+    apply app_closed_iff.mpr
+    have .app _ _ t' htf hte := ht
+    dsimp only at *
+    constructor
+    · exact closed_of_step htp.validRefs htf.validRefs hcf hs
+    · exact ih hce htp hte
+  | condT p et ef =>
+    obtain ⟨-, hcet, -⟩ := cond_closed_iff.mp hc
+    exact hcet
+  | condF p et ef =>
+    obtain ⟨-, -, hcef⟩ := cond_closed_iff.mp hc
+    exact hcef
+  | condC p p' c c' et ef hs ih =>
+    obtain ⟨hcc, hcet, hcef⟩ := cond_closed_iff.mp hc
+    apply cond_closed_iff.mpr
+    have .cond _ _ _ _ htc htet htef := ht
+    and_intros
+    · exact ih hcc htp htc
+    · apply closed_of_step htp.validRefs htet.validRefs hcet
+      exact (.condC _ _ _ _ _ _ hs)
+    · apply closed_of_step htp.validRefs htef.validRefs hcef
+      exact (.condC _ _ _ _ _ _ hs)
